Hide the proofs in the IndexedBagAsBag typeclass implementation
Proving the various lemmas separately solves the performance problem
observed when calling Defined in TreeBasedRefinement.v.

ADTExamples/QueryStructure/Bags/Bags.v
@@ -29,6 +29,37 @@ Qed.
 
 Require Import SetEq.
 
+Definition BagInsertEnumerate
+           {TContainer TItem: Type}
+           (benumerate : TContainer -> list TItem)
+           (binsert    : TContainer -> TItem -> TContainer) :=
+  forall item inserted container,
+    List.In item (benumerate (binsert container inserted)) <->
+    List.In item (benumerate container) \/ item = inserted.
+    
+Definition BagEnumerateEmpty
+           {TContainer TItem: Type}
+           (benumerate : TContainer -> list TItem)
+           (bempty     : TContainer) :=
+  forall item, ~ List.In item (benumerate bempty).
+
+Definition BagFindStar
+           {TContainer TItem TSearchTerm: Type}
+           (bfind : TContainer -> TSearchTerm -> list TItem)
+           (benumerate : TContainer -> list TItem)
+           (bstar : TSearchTerm) :=
+  forall container, bfind container bstar = benumerate container.
+
+Definition BagFindCorrect
+           {TContainer TItem TSearchTerm: Type}
+           (bfind         : TContainer -> TSearchTerm -> list TItem)
+           (bfind_matcher : TSearchTerm -> TItem -> bool)
+           (benumerate : TContainer -> list TItem) :=
+  forall container search_term,
+    SetEq
+      (List.filter (bfind_matcher search_term) (benumerate container))
+      (bfind container search_term).
+
 Class Bag (TContainer TItem TSearchTerm: Type) :=
   {
     bempty        : TContainer;
@@ -39,15 +70,10 @@ Class Bag (TContainer TItem TSearchTerm: Type) :=
     bfind      : TContainer -> TSearchTerm -> list TItem;
     binsert    : TContainer -> TItem -> TContainer;
     
-    binsert_enumerate : forall item inserted container,
-                          List.In item (benumerate (binsert container inserted)) <->
-                          List.In item (benumerate container) \/ item = inserted;
-    benumerate_empty  : forall item, ~ List.In item (benumerate bempty);
-    bstar_search      : forall container, bfind container bstar = benumerate container;
-    bfind_correct     : forall container search_term,
-                          SetEq
-                            (List.filter (bfind_matcher search_term) (benumerate container))
-                            (bfind container search_term)
+    binsert_enumerate : BagInsertEnumerate benumerate binsert;
+    benumerate_empty  : BagEnumerateEmpty benumerate bempty;
+    bfind_star        : BagFindStar bfind benumerate bstar;
+    bfind_correct     : BagFindCorrect bfind bfind_matcher benumerate
   }.
 
 Record BagPlusBagProof {TItem} :=
@@ -102,432 +128,563 @@ Module IndexedTree (Import M: WS).
 
   Lemma iconsistency_empty :
     forall {TBag TItem TBagSearchTerm: Type} 
-           {bags_bag: Bag TBag TItem TBagSearchTerm} {projection},
+           {bags_bag: Bag TBag TItem TBagSearchTerm} 
+           projection,
       IndexedBagConsistency projection (empty TBag).
   Proof.
       unfold IndexedBagConsistency; 
       intros; rewrite empty_mapsto_iff in *; exfalso; trivial.
   Qed.
 
-    Lemma consistency_key_eq :
-      forall {TBag TItem TBagSearchTerm},
-      forall bags_bag (projection: TItem -> TKey),
-      forall (indexed_bag: @IndexedBag TBag TItem TBagSearchTerm bags_bag projection),
-      forall (key: TKey) bag item,
-        MapsTo key bag (ifmap indexed_bag) ->
-        List.In item (benumerate bag) ->
-        E.eq (projection item) key.
-    Proof.
-      intros.
-      destruct indexed_bag as [? consistent].
-      unfold IndexedBagConsistency in consistent.
-      eapply consistent; eauto.
-    Qed.
+  Lemma consistency_key_eq :
+    forall {TBag TItem TBagSearchTerm},
+    forall bags_bag (projection: TItem -> TKey),
+    forall (indexed_bag: @IndexedBag TBag TItem TBagSearchTerm bags_bag projection),
+    forall (key: TKey) bag item,
+      MapsTo key bag (ifmap indexed_bag) ->
+      List.In item (benumerate bag) ->
+      E.eq (projection item) key.
+  Proof.
+    intros.
+    destruct indexed_bag as [? consistent].
+    unfold IndexedBagConsistency in consistent.
+    eapply consistent; eauto.
+  Qed.
 
-    Ltac destruct_if :=
-      match goal with
-          [ |- context [ if ?cond then _ else _ ] ] => destruct cond
-      end.
+  Ltac destruct_if :=
+    match goal with
+        [ |- context [ if ?cond then _ else _ ] ] => destruct cond
+    end.
 
-    Lemma KeyFilter_true :
-      forall {A} k projection (item: A),
-        KeyFilter k projection item = true <-> E.eq (projection item) k.
-    Proof.
-      unfold KeyFilter; intros;
-      destruct_if; intros; intuition.
-    Qed.
+  Lemma KeyFilter_true :
+    forall {A} k projection (item: A),
+      KeyFilter k projection item = true <-> E.eq (projection item) k.
+  Proof.
+    unfold KeyFilter; intros;
+    destruct_if; intros; intuition.
+  Qed.
 
-    Lemma KeyFilter_false :
-      forall {A} k projection (item: A),
-        KeyFilter k projection item = false <-> ~ E.eq (projection item) k.
-    Proof.
-      unfold KeyFilter; intros;
-      destruct_if; intros; intuition.
-    Qed.
+  Lemma KeyFilter_false :
+    forall {A} k projection (item: A),
+      KeyFilter k projection item = false <-> ~ E.eq (projection item) k.
+  Proof.
+    unfold KeyFilter; intros;
+    destruct_if; intros; intuition.
+  Qed.
 
-    Instance IndexedBagAsBag 
-             (TBag TItem TBagSearchTerm: Type) 
-             (bags_bag: Bag TBag TItem TBagSearchTerm) projection 
-    : Bag 
-        (@IndexedBag TBag TItem TBagSearchTerm bags_bag projection) 
-        TItem 
-        ((option TKey) * TBagSearchTerm) :=
-      {| 
-        bempty := {| ifmap        := empty TBag;
-                     iconsistency := iconsistency_empty |};
+  Definition IndexedBag_bempty 
+             {TBag TItem TBagSearchTerm: Type}
+             {bags_bag: Bag TBag TItem TBagSearchTerm}
+             (projection: TItem -> TKey) :=
+    {| ifmap        := empty TBag;
+       iconsistency := iconsistency_empty projection |}.
 
-        bstar  := (None, @bstar _ _ _ bags_bag);
+  Definition IndexedBag_bstar
+             {TBag TItem TBagSearchTerm: Type}
+             {bags_bag: Bag TBag TItem TBagSearchTerm} :=
+    (@None TKey, @bstar _ _ _ bags_bag).
 
-        bfind_matcher key_searchterm item :=
-          let (key_option, search_term) := key_searchterm in
-          match key_option with
-            | Some k => KeyFilter k projection item
-            | None   => true 
-          end && (bfind_matcher search_term item);
 
-        benumerate container :=
-          flatten (List.map benumerate (Values (container.(ifmap))));
+  Definition IndexedBag_bfind_matcher 
+             {TBag TItem TBagSearchTerm: Type}
+             {bags_bag: Bag TBag TItem TBagSearchTerm}
+             (projection: TItem -> TKey)
+             (key_searchterm: (option TKey) * TBagSearchTerm) (item: TItem) :=
+    let (key_option, search_term) := key_searchterm in
+    match key_option with
+      | Some k => KeyFilter k projection item
+      | None   => true 
+    end && (bfind_matcher search_term item).
 
-        bfind container key_searchterm :=
-          let (key_option, search_term) := key_searchterm in
-          match key_option with
-            | Some k =>
-              match find k container.(ifmap) with
-                | Some bag => bag.(bfind) search_term
-                | None     => []
-              end
-            | None   =>
-              flatten (List.map (fun bag => bag.(bfind) search_term) (Values container.(ifmap)))
-          end;
+  Definition IndexedBag_benumerate 
+             {TBag TItem TBagSearchTerm: Type}
+             {bags_bag: Bag TBag TItem TBagSearchTerm}
+             {projection: TItem -> TKey} 
+             (container: @IndexedBag TBag TItem TBagSearchTerm bags_bag projection) :=
+    flatten (List.map benumerate (Values (ifmap container))).
 
-        binsert container item :=
-          let k := projection item in
-          let bag := FindWithDefault k bempty container.(ifmap) in
-          {|
-            ifmap := add k (bag.(binsert) item) container.(ifmap);
-            iconsistency := _
-          |}
-      |}. 
-    Proof.
-      intros; simpl in *.
+  Definition IndexedBag_bfind
+             {TBag TItem TBagSearchTerm: Type}
+             {bags_bag: Bag TBag TItem TBagSearchTerm}
+             (projection: TItem -> TKey)
+             (container: @IndexedBag TBag TItem TBagSearchTerm bags_bag projection) 
+             (key_searchterm: (option TKey) * TBagSearchTerm) :=
+    let (key_option, search_term) := key_searchterm in
+    match key_option with
+      | Some k =>
+        match find k (ifmap container) with
+          | Some bag => @bfind _ _ _ bags_bag bag search_term
+          | None     => []
+        end
+      | None   =>
+        flatten (List.map (fun bag =>  @bfind _ _ _ bags_bag bag search_term) (Values (ifmap container)))
+    end.
 
-      unfold Values.
-      setoid_rewrite in_flatten_iff.
-      setoid_rewrite in_map_iff.
-      setoid_rewrite <- MapsTo_snd.
+  Lemma indexed_bag_insert_consistent :
+    forall {TBag TItem TBagSearchTerm: Type}
+           {bags_bag: Bag TBag TItem TBagSearchTerm}
+           {projection: TItem -> TKey} 
+           (container: @IndexedBag TBag TItem TBagSearchTerm bags_bag projection) 
+           (item: TItem),
+      let k := projection item in
+      let fmap := ifmap container in
+      let bag := FindWithDefault k bempty fmap in
+      IndexedBagConsistency projection (add k (binsert bag item) fmap).
+  Proof.
+    intros.
 
-      split; intro H.
-      
-      destruct H as [ items ( in_seq & [ bag (bag_items & [ key maps_to ]) ] ) ].
-      pose proof maps_to as maps_to'.
-      rewrite add_mapsto_iff in maps_to;
-        destruct maps_to as [(is_eq & refreshed) | (neq & maps_to)].
+    intros k' bag' maps_to item'.
 
+    rewrite add_mapsto_iff in maps_to;
+      destruct maps_to as [(is_eq & refreshed) | (neq & maps_to)];
       subst.
-      rewrite binsert_enumerate in in_seq.
-      destruct in_seq as [ in_seq | ? ]; eauto.
-      left.
-      
-      Ltac autoexists :=
-        repeat progress match goal with
-                          | [ |- exists _, _ ] => eexists; autoexists
-                          | [ |- ?a = ?b ]     => first [ (has_evar a; has_evar b; idtac) | eauto]
-                          | [ |- E.eq _ _ ]    => eauto
-                          | [ |- _ /\ _ ]      => split; autoexists
-                          | [ |- _ \/ _ ]      => left; autoexists
-                        end.
-      
-      destruct (FindWithDefault_dec (projection inserted) bempty (ifmap container)) 
-        as [ [result (mapsto & equality)] | (not_found & equality) ];
-        rewrite equality in *; clear equality.
-      
-      autoexists; eauto.
-      
-      exfalso; apply benumerate_empty in in_seq; tauto.
 
-      autoexists; eauto.
+    rewrite (binsert_enumerate item' item bag).
+    intro H; destruct H.
+    apply (iconsistency container k' bag); trivial.    
 
-      Focus 2.
-      unfold flatten; simpl.
-      rewrite Values_empty; tauto.
- 
-      destruct H as [ [ items ( in_seq & [ bag ( bag_items & [ key maps_to ] ) ] ) ] | eq_item_inserted ].
-      
-      pose proof maps_to as maps_to'.
-      apply (iconsistency container) in maps_to.    
-      setoid_rewrite bag_items in maps_to.
-      specialize (maps_to item in_seq).
-      
-      setoid_rewrite add_mapsto_iff.
+    rewrite <- is_eq.
+    unfold bag in *.
 
-      destruct (E.eq_dec (projection inserted) key);
-        try solve [ repeat (eexists; split; eauto) ].
-      
-      autoexists.
+    unfold fmap in *.
+    destruct (FindWithDefault_dec k (@bempty _ _ _ bags_bag) (ifmap container))
+      as [ [bag' (mapsto & equality)] | (not_found & equality) ];
+      rewrite equality in *; clear equality.
 
-      apply binsert_enumerate.
+    subst; trivial.
+    exfalso; apply (@benumerate_empty _ _ _ bags_bag) in H; trivial.
+    
+    subst.
+    unfold k in *. 
+    trivial.
 
-      destruct (FindWithDefault_dec (projection inserted) bempty (ifmap container))
-        as [ [bag' (mapsto & equality)] | (not_found & equality) ];
-        rewrite equality in *; clear equality.
+    apply (iconsistency container k' bag' maps_to item').
+  Qed.    
 
-      rewrite e in mapsto.
-      pose proof (MapsTo_fun mapsto maps_to') as bag'_bag.
-      rewrite bag'_bag.
-      rewrite bag_items.
-      auto.
+  Definition IndexedBag_binsert 
+             {TBag TItem TBagSearchTerm: Type}
+             {bags_bag: Bag TBag TItem TBagSearchTerm}
+             (projection: TItem -> TKey)
+             (container: @IndexedBag TBag TItem TBagSearchTerm bags_bag projection) 
+             (item: TItem) : @IndexedBag TBag TItem TBagSearchTerm bags_bag projection :=
+    let k := projection item in
+    let fmap := ifmap container in
+    let bag := FindWithDefault k bempty fmap in
+    {|
+      ifmap := add k (binsert bag item) fmap;
+      iconsistency := indexed_bag_insert_consistent container item
+    |}.
 
-      rewrite find_mapsto_iff in maps_to'.
-      rewrite <- e in maps_to'.
-      match goal with 
-        | [ H: ?a = Some ?b, H': ?a = None |- _ ] => assert (Some b = None) by (transitivity a; auto); discriminate
-      end.
+  Lemma IndexedBag_BagInsertEnumerate :
+    forall {TBag TItem TBagSearchTerm: Type}
+           {bags_bag: Bag TBag TItem TBagSearchTerm}
+           (projection: TItem -> TKey),
+      BagInsertEnumerate IndexedBag_benumerate (IndexedBag_binsert projection).
+  Proof.
 
-      subst item.
-      match goal with
-        | [ |- context [ add ?key ?value ?container ] ] => set (k := key); set (v := value)
-      end.
+    unfold BagInsertEnumerate, Values, IndexedBag_benumerate.
+    intros; simpl in *.
 
-      exists (benumerate v).
+    setoid_rewrite in_flatten_iff.
+    setoid_rewrite in_map_iff.
+    setoid_rewrite <- MapsTo_snd.
 
-      split.
+    split; intro H.
+    
+    destruct H as [ items ( in_seq & [ bag (bag_items & [ key maps_to ]) ] ) ].
+    pose proof maps_to as maps_to'.
+    rewrite add_mapsto_iff in maps_to;
+      destruct maps_to as [(is_eq & refreshed) | (neq & maps_to)].
 
-      unfold v.
-      rewrite binsert_enumerate; auto.
+    subst.
+    rewrite (binsert_enumerate _) in in_seq.
+    destruct in_seq as [ in_seq | ? ]; eauto.
+    left.
+    
+    Ltac autoexists :=
+      repeat progress match goal with
+                        | [ |- exists _, _ ] => eexists; autoexists
+                        | [ |- ?a = ?b ]     => first [ (has_evar a; has_evar b; idtac) | eauto]
+                        | [ |- E.eq _ _ ]    => eauto
+                        | [ |- _ /\ _ ]      => split; autoexists
+                        | [ |- _ \/ _ ]      => left; autoexists
+                      end.
+    
+    destruct (FindWithDefault_dec (projection inserted) bempty (ifmap container)) 
+      as [ [result (mapsto & equality)] | (not_found & equality) ];
+      rewrite equality in *; clear equality.
+    
+    autoexists; eauto.
+    
+    exfalso; apply benumerate_empty in in_seq; tauto.
 
-      exists v; split; trivial.
-      exists k.
-      apply add_1; trivial.
+    autoexists; eauto.
 
-      intros; induction (Values (ifmap container)); simpl; trivial.
-      rewrite (@bstar_search _ _ _ bags_bag).
-      f_equal; trivial.
+    destruct H as [ [ items ( in_seq & [ bag ( bag_items & [ key maps_to ] ) ] ) ] | eq_item_inserted ].
+    
+    pose proof maps_to as maps_to'.
+    apply (iconsistency container) in maps_to.    
+    setoid_rewrite bag_items in maps_to.
+    specialize (maps_to item in_seq).
+    
+    setoid_rewrite add_mapsto_iff.
 
+    destruct (E.eq_dec (projection inserted) key);
+      try solve [ repeat (eexists; split; eauto) ].
+    
+    autoexists.
 
+    apply binsert_enumerate.
+
+    destruct (FindWithDefault_dec (projection inserted) bempty (ifmap container))
+      as [ [bag' (mapsto & equality)] | (not_found & equality) ];
+      rewrite equality in *; clear equality.
+
+    rewrite e in mapsto.
+    pose proof (MapsTo_fun mapsto maps_to') as bag'_bag.
+    rewrite bag'_bag.
+    rewrite bag_items.
+    auto.
+
+    rewrite find_mapsto_iff in maps_to'.
+    rewrite <- e in maps_to'.
+    match goal with 
+      | [ H: ?a = Some ?b, H': ?a = None |- _ ] => assert (Some b = None) by (transitivity a; auto); discriminate
+    end.
+
+    subst item.
+    match goal with
+      | [ |- context [ add ?key ?value ?container ] ] => set (k := key); set (v := value)
+    end.
+
+    exists (benumerate v).
+
+    split.
+
+    unfold v.
+    rewrite (binsert_enumerate _); auto.
+
+    exists v; split; trivial.
+    exists k.
+    apply add_1; trivial.
+  Qed.
+
+  Lemma IndexedBag_BagEnumerateEmpty :
+    forall {TBag TItem TBagSearchTerm: Type}
+           {bags_bag: Bag TBag TItem TBagSearchTerm}
+           (projection: TItem -> TKey),
+      BagEnumerateEmpty IndexedBag_benumerate (IndexedBag_bempty projection).
+  Proof.
+    intros;
+    unfold BagEnumerateEmpty, IndexedBag_benumerate, flatten; simpl;
+    rewrite Values_empty; tauto.
+  Qed.
+
+  Lemma IndexedBag_BagFindStar :
+    forall {TBag TItem TBagSearchTerm: Type}
+           {bags_bag: Bag TBag TItem TBagSearchTerm}
+           (projection: TItem -> TKey),
+      BagFindStar (IndexedBag_bfind projection) IndexedBag_benumerate IndexedBag_bstar.
+  Proof.
+    unfold BagFindStar, IndexedBag_benumerate; simpl.
+    
+    intros; induction (Values (ifmap container)); simpl; trivial.
+    rewrite (@bfind_star _ _ _ bags_bag).
+    f_equal; trivial.
+  Qed.
+
+  Lemma IndexedBag_BagFindCorrect :
+    forall {TBag TItem TBagSearchTerm: Type}
+           {bags_bag: Bag TBag TItem TBagSearchTerm}
+           (projection: TItem -> TKey),
+      BagFindCorrect (IndexedBag_bfind projection)
+                     (IndexedBag_bfind_matcher projection) IndexedBag_benumerate.
+  Proof.
+    intros.
+    destruct search_term as (option_key, search_term).
+    destruct option_key as [ key | ].
+
+    (* Key provided *)
+
+    unfold IndexedBag_benumerate, IndexedBag_bfind_matcher.
+    pose (iconsistency container).
+    unfold IndexedBagConsistency in i.
+
+    rewrite filter_and'.
+
+    rewrite flatten_filter.
+    
+    Lemma consist :
+      forall 
+        {TBag TItem TSearchTerm bags_bag projection} 
+        (container: @IndexedBag TBag TItem TSearchTerm bags_bag projection),
+      forall k,
+        eq
+          (flatten
+             (List.map (List.filter (KeyFilter k projection))
+                       (List.map benumerate (Values (ifmap container)))))
+          match find k (ifmap container) with
+            | Some bag => benumerate bag
+            | None => []
+          end.
+    Proof.          
       intros.
-      destruct search_term as (option_key, search_term).
-      destruct option_key as [ key | ].
 
-      (* Key provided *)
+      pose (iconsistency container); unfold IndexedBagConsistency in i.
+      unfold Values.
+      destruct (find k (ifmap container)) as [ bag | ] eqn:eqfind.
 
-      pose (iconsistency container).
-      unfold IndexedBagConsistency in i.
+      rewrite <- find_mapsto_iff in eqfind.
+      (* assert (exists k', MapsTo k' bag (ifmap container)) as eqfind' by (exists k; trivial).*)
 
+      pose proof eqfind as maps_to.
 
-      rewrite filter_and'.
+      rewrite elements_mapsto_iff in eqfind.
+      apply InA_split in eqfind.
 
-      rewrite flatten_filter.
+      destruct eqfind as [ l1 [ y [ l2 (y_k_bag & decomp) ] ] ].
+      rewrite decomp.
       
-      Lemma consist :
-        forall 
-          {TBag TItem TSearchTerm bags_bag projection} 
-          (container: @IndexedBag TBag TItem TSearchTerm bags_bag projection),
-        forall k,
-          eq
-            (flatten
-               (List.map (List.filter (KeyFilter k projection))
-                         (List.map benumerate (Values (ifmap container)))))
-            match find k (ifmap container) with
-              | Some bag => benumerate bag
-              | None => []
-            end.
-      Proof.          
-        intros.
-        
-        pose (iconsistency container); unfold IndexedBagConsistency in i.
-        unfold Values.
-        destruct (find k (ifmap container)) as [ bag | ] eqn:eqfind.
+      rewrite (map_map snd benumerate).
+      rewrite ! map_app; simpl.
+      
+      pose proof (elements_3w (ifmap container)) as no_dup.
+      rewrite decomp in no_dup; apply NoDupA_swap in no_dup; eauto using equiv_eq_key.
 
-        rewrite <- find_mapsto_iff in eqfind.
-        (* assert (exists k', MapsTo k' bag (ifmap container)) as eqfind' by (exists k; trivial).*)
+      inversion no_dup as [ | ? ? y_not_in no_dup' ]; subst.
+      rewrite InA_app_iff in y_not_in by eauto using equiv_eq_key.
+      
+      unfold eq_key_elt in y_k_bag; simpl in y_k_bag.
+      destruct y_k_bag as (y_k & y_bag).
 
-        pose proof eqfind as maps_to.
+      assert (forall k' bag', InA (@eq_key_elt _) (k', bag') (l1 ++ l2) -> 
+                              forall item, 
+                                List.In item (benumerate bag') ->
+                                ~ E.eq (projection item) k).
+      {
+        intros k' bag' in_app item in_bag'_items eq_k.
 
-        rewrite elements_mapsto_iff in eqfind.
-        apply InA_split in eqfind.
+        rewrite InA_app_iff in in_app; eauto using equiv_eq_key_elt.
+        pose proof in_app as in_app'.
 
-        destruct eqfind as [ l1 [ y [ l2 (y_k_bag & decomp) ] ] ].
-        rewrite decomp.
-        
-        rewrite (map_map snd benumerate).
-        rewrite ! map_app; simpl.
-        
-        pose proof (elements_3w (ifmap container)) as no_dup.
-        rewrite decomp in no_dup; apply NoDupA_swap in no_dup; eauto using equiv_eq_key.
+        apply (InA_front_tail_InA _ _ y) in in_app.
+        rewrite <- decomp, <- elements_mapsto_iff in in_app.
 
-        inversion no_dup as [ | ? ? y_not_in no_dup' ]; subst.
-        rewrite InA_app_iff in y_not_in by eauto using equiv_eq_key.
-     
-        unfold eq_key_elt in y_k_bag; simpl in y_k_bag.
-        destruct y_k_bag as (y_k & y_bag).
+        pose proof (i _ _ in_app _ in_bag'_items) as eq_k'. 
+        symmetry in eq_k.
+        pose proof (E.eq_trans eq_k eq_k').
 
-        assert (forall k' bag', InA (@eq_key_elt _) (k', bag') (l1 ++ l2) -> 
-                                   forall item, 
-                                     List.In item (benumerate bag') ->
-                                     ~ E.eq (projection item) k).
-        {
-          intros k' bag' in_app item in_bag'_items eq_k.
+        assert (eq_key y (k', bag')) as y_eq by (unfold eq_key; simpl; eauto).
 
-          rewrite InA_app_iff in in_app; eauto using equiv_eq_key_elt.
-          pose proof in_app as in_app'.
+        destruct in_app' as [ in_seq | in_seq ];
+          (apply (InA_eqke_eqk (k2 := fst y) (snd y)) in in_seq; eauto);
+          rewrite <- surjective_pairing in in_seq; intuition.
+      }
 
-          apply (InA_front_tail_InA _ _ y) in in_app.
-          rewrite <- decomp, <- elements_mapsto_iff in in_app.
+      Lemma In_InA :
+        forall (A : Type) (l : list A) (eqA : relation A) (x : A),
+          Equivalence eqA -> List.In x l -> InA eqA x l.
+      Proof.
+        induction l; intros; simpl in *.
+        exfalso; eauto using in_nil.
+        destruct H0.
+        apply InA_cons_hd; subst; reflexivity.
+        apply InA_cons_tl, IHl; trivial.
+      Qed.
 
-          pose proof (i _ _ in_app _ in_bag'_items) as eq_k'. 
-          symmetry in eq_k.
-          pose proof (E.eq_trans eq_k eq_k').
+      rewrite ! map_filter_all_false;
+        [ | intros subseq in_map item in_subseq;
+            rewrite in_map_iff in in_map;
+            destruct in_map as [ (k', bag') (benum_eq & in_seq) ];
+            rewrite KeyFilter_false;
+            
+            simpl in benum_eq;
+            subst subseq;
+            apply (H k' bag'); 
+            eauto;
+            
+            apply In_InA; eauto using equiv_eq_key_elt;
+            rewrite in_app_iff;
+            eauto 
+              .. ].
 
-          assert (eq_key y (k', bag')) as y_eq by (unfold eq_key; simpl; eauto).
+      rewrite 
+        flatten_app, 
+      flatten_head, 
+      !flatten_nils, 
+      app_nil_l, app_nil_r, 
+      <- y_bag,
+      filter_all_true; trivial.
 
-          destruct in_app' as [ in_seq | in_seq ];
-            (apply (InA_eqke_eqk (k2 := fst y) (snd y)) in in_seq; eauto);
-            rewrite <- surjective_pairing in in_seq; intuition.
-        }
-
-        Lemma In_InA :
-          forall (A : Type) (l : list A) (eqA : relation A) (x : A),
-            Equivalence eqA -> List.In x l -> InA eqA x l.
-        Proof.
-          induction l; intros; simpl in *.
-          exfalso; eauto using in_nil.
-          destruct H0.
-          apply InA_cons_hd; subst; reflexivity.
-          apply InA_cons_tl, IHl; trivial.
-        Qed.
-
-        rewrite ! map_filter_all_false;
-          [ | intros subseq in_map item in_subseq;
-              rewrite in_map_iff in in_map;
-              destruct in_map as [ (k', bag') (benum_eq & in_seq) ];
-              rewrite KeyFilter_false;
-              
-              simpl in benum_eq;
-              subst subseq;
-              apply (H k' bag'); 
-              eauto;
-              
-              apply In_InA; eauto using equiv_eq_key_elt;
-              rewrite in_app_iff;
-              eauto 
-                .. ].
-
-        rewrite 
-          flatten_app, 
-          flatten_head, 
-          !flatten_nils, 
-          app_nil_l, app_nil_r, 
-          <- y_bag,
-          filter_all_true; trivial.
-
-        intros;
+      intros;
         rewrite KeyFilter_true;
         apply (iconsistency container _ bag); eauto.
 
-        Lemma nil_in_false :
-          forall {A} seq,
-            seq = [] <-> ~ exists (x: A), List.In x seq.
-        Proof.
-          split; intro H.
-          intros [ x in_seq ]; subst; eauto using in_nil.
-          destruct seq as [ | a ]; trivial.
-          exfalso; apply H; exists a; simpl; intuition.
-        Qed.
-        
-        rewrite nil_in_false.
-        intros [item item_in].
-
-        rewrite in_flatten_iff in item_in.
-        do 2 setoid_rewrite in_map_iff in item_in.
-
-        destruct item_in as 
-            [ subseq 
-                (in_subseq 
-                   & [ subseq_prefilter 
-                         ( pre_post_filter 
-                             & [ bag 
-                                   (eq_bag_pre_filter 
-                                      & bag_in) ] ) ] ) ].
-
-        subst subseq.
-        rewrite filter_In in in_subseq.
-        destruct in_subseq as (in_subseq_prefilter & key_filter).
-
-        rewrite KeyFilter_true in key_filter.
-        rewrite <- MapsTo_snd in bag_in.
-        destruct bag_in as [k' maps_to].
-
-        subst.
-        rewrite <- key_filter in eqfind.
-        rewrite <- (iconsistency container k' bag maps_to _ in_subseq_prefilter) in maps_to.
-        rewrite find_mapsto_iff in maps_to.
-
-        congruence.
-      Qed.
-
-      rewrite consist.
-      destruct (find key (ifmap container)) as [ bag | ].
-
-      apply bfind_correct.
-      eauto using SetEq_Reflexive.
-
-      (* No key provided *)
-
-      rewrite flatten_filter.
-
-      induction (Values (ifmap container)); simpl.
-
-      compute; tauto.
-
-      rewrite IHl.
-
-      Lemma SetEq_app :
-        forall {A: Type} (s1 t1 s2 t2: list A),
-          (SetEq s1 s2) /\ (SetEq t1 t2) -> SetEq (s1 ++ t1) (s2 ++ t2).
+      Lemma nil_in_false :
+        forall {A} seq,
+          seq = [] <-> ~ exists (x: A), List.In x seq.
       Proof.
-        unfold SetEq; 
-        intros A s1 t1 s2 t2 (s1s2 & t1t2); 
-        split;
-        rewrite ! in_app_iff;
-        intro inApp;
-        [ rewrite s1s2, t1t2 in inApp
-        | rewrite <- s1s2, <- t1t2 in inApp ];
-        trivial.
+        split; intro H.
+        intros [ x in_seq ]; subst; eauto using in_nil.
+        destruct seq as [ | a ]; trivial.
+        exfalso; apply H; exists a; simpl; intuition.
       Qed.
-
-      apply SetEq_app; split; eauto using SetEq_Reflexive.
-      apply bfind_correct.
-
-      Grab Existential Variables.
-      intros k' bag' maps_to item'.
-
-      rewrite add_mapsto_iff in maps_to;
-        destruct maps_to as [(is_eq & refreshed) | (neq & maps_to)];
-        subst.
-
-      rewrite binsert_enumerate.
-      intro H; destruct H.
-      apply (iconsistency container k' bag); trivial.    
-
-      rewrite <- is_eq.
-      unfold bag in *.
-
-      destruct (FindWithDefault_dec k bempty (ifmap container))
-        as [ [bag' (mapsto & equality)] | (not_found & equality) ];
-        rewrite equality in *; clear equality.
-
-      subst; trivial.
-      exfalso; apply benumerate_empty in H; trivial.
       
-      subst.
-      unfold k in *. 
-      trivial.
+      rewrite nil_in_false.
+      intros [item item_in].
 
-      apply (iconsistency container k' bag' maps_to item').
-    Defined.
+      rewrite in_flatten_iff in item_in.
+      do 2 setoid_rewrite in_map_iff in item_in.
+
+      destruct item_in as 
+          [ subseq 
+              (in_subseq 
+                 & [ subseq_prefilter 
+                       ( pre_post_filter 
+                           & [ bag 
+                                 (eq_bag_pre_filter 
+                                    & bag_in) ] ) ] ) ].
+
+      subst subseq.
+      rewrite filter_In in in_subseq.
+      destruct in_subseq as (in_subseq_prefilter & key_filter).
+
+      rewrite KeyFilter_true in key_filter.
+      rewrite <- MapsTo_snd in bag_in.
+      destruct bag_in as [k' maps_to].
+
+      subst.
+      rewrite <- key_filter in eqfind.
+      rewrite <- (iconsistency container k' bag maps_to _ in_subseq_prefilter) in maps_to.
+      rewrite find_mapsto_iff in maps_to.
+
+      congruence.
+    Qed.
+
+    simpl.
+    rewrite consist.
+    destruct (find key (ifmap container)) as [ bag | ].
+
+    apply bfind_correct.
+    eauto using SetEq_Reflexive.
+
+    (* No key provided *)
+
+    simpl. unfold IndexedBag_benumerate, IndexedBag_bfind_matcher.
+    rewrite flatten_filter.
+
+    induction (Values (ifmap container)); simpl.
+
+    compute; tauto.
+
+    rewrite IHl.
+
+    Lemma SetEq_app :
+      forall {A: Type} (s1 t1 s2 t2: list A),
+        (SetEq s1 s2) /\ (SetEq t1 t2) -> SetEq (s1 ++ t1) (s2 ++ t2).
+    Proof.
+      unfold SetEq; 
+      intros A s1 t1 s2 t2 (s1s2 & t1t2); 
+      split;
+      rewrite ! in_app_iff;
+      intro inApp;
+      [ rewrite s1s2, t1t2 in inApp
+      | rewrite <- s1s2, <- t1t2 in inApp ];
+      trivial.
+    Qed.
+
+    apply SetEq_app; split; eauto using SetEq_Reflexive.
+    apply bfind_correct.
+  Qed.
+  
+  Instance IndexedBagAsBag 
+           (TBag TItem TBagSearchTerm: Type) 
+           (bags_bag: Bag TBag TItem TBagSearchTerm) (projection: TItem -> TKey) 
+  : Bag 
+      (@IndexedBag TBag TItem TBagSearchTerm bags_bag projection) 
+      TItem 
+      ((option TKey) * TBagSearchTerm) :=
+    {| 
+      bempty        := IndexedBag_bempty projection;
+      bstar         := IndexedBag_bstar;
+      bfind_matcher := IndexedBag_bfind_matcher projection;
+
+      benumerate := IndexedBag_benumerate;
+      bfind      := IndexedBag_bfind projection;
+      binsert    := IndexedBag_binsert projection;
+
+      binsert_enumerate := IndexedBag_BagInsertEnumerate projection;
+      benumerate_empty  := IndexedBag_BagEnumerateEmpty projection;
+      bfind_star        := IndexedBag_BagFindStar projection;
+      bfind_correct     := IndexedBag_BagFindCorrect projection
+    |}. 
 End IndexedTree.
+
+Definition ListAsBag_bfind 
+           {TItem TSearchTerm: Type}
+           (matcher: TSearchTerm -> TItem -> bool) 
+           (container: list TItem) (search_term: TSearchTerm) :=
+  List.filter (matcher search_term) container.
+
+Definition ListAsBag_binsert 
+           {TItem: Type}
+           (container: list TItem) 
+           (item: TItem) :=
+  cons item container.
+
+Lemma List_BagInsertEnumerate :
+  forall {TItem: Type},
+  BagInsertEnumerate id (ListAsBag_binsert (TItem := TItem)).
+Proof.
+  firstorder.
+Qed.
+
+Lemma List_BagFindStar :
+  forall {TItem TSearchTerm: Type}
+         (star: TSearchTerm)
+         (matcher: TSearchTerm -> TItem -> bool)
+         (find_star: forall (i: TItem), matcher star i = true),
+  BagFindStar (ListAsBag_bfind matcher) id star.
+Proof.
+  intros;
+  induction container; simpl; 
+  [ | rewrite find_star, IHcontainer]; trivial.
+Qed.
+
+Lemma List_BagEnumerateEmpty :
+  forall {TItem: Type},
+    BagEnumerateEmpty id (@nil TItem).
+Proof.
+  firstorder.
+Qed.
+  
+Lemma List_BagFindCorrect :
+  forall {TItem TSearchTerm: Type}
+         (matcher: TSearchTerm -> TItem -> bool),
+         BagFindCorrect (ListAsBag_bfind matcher) matcher id.
+Proof.
+  firstorder.
+Qed.
 
 Instance ListAsBag
          {TItem TSearchTerm: Type}
          (star: TSearchTerm)
          (matcher: TSearchTerm -> TItem -> bool)
-         (star_search: forall (i: TItem), matcher star i = true)
-: Bag (list TItem) TItem TSearchTerm.
-Proof.
-  refine (
-      {| 
-        bempty := [];
-        bstar  := star;
-        benumerate := id;
-        bfind container search_term := List.filter (matcher search_term) container;
-        binsert container item := cons item container
-      |}
-    ); simpl in *; intuition.
-
-  unfold id.
-  induction container; simpl; trivial.
-  rewrite star_search, IHcontainer; trivial.
-Defined.
+         (find_star: forall (i: TItem), matcher star i = true)
+: Bag (list TItem) TItem TSearchTerm :=
+  {| 
+    bempty := [];
+    bstar  := star;
+    
+    benumerate := id;
+    bfind      := ListAsBag_bfind matcher;
+    binsert    := ListAsBag_binsert;
+    
+    binsert_enumerate := List_BagInsertEnumerate;
+    benumerate_empty  := List_BagEnumerateEmpty;
+    bfind_star        := List_BagFindStar star matcher find_star;
+    bfind_correct     := List_BagFindCorrect matcher
+  |}.
 
 Definition IsCacheable
            {TItem TAcc}
@@ -537,7 +694,7 @@ Definition IsCacheable
     SetEq seq1 seq2 ->
     (List.fold_right cache_updater initial_value seq1 =
      List.fold_right cache_updater initial_value seq2).
-  
+
 Record CachingBag 
        {TBag TItem TSearchTerm: Type} 
        {bag_bag: Bag TBag TItem TSearchTerm} 
@@ -572,7 +729,8 @@ Qed.
 Lemma benumerate_empty_eq_nil {TContainer TItem TSearchTerm} (bag: Bag TContainer TItem TSearchTerm):
   (benumerate bempty) = []. 
 Proof.
-  pose proof (benumerate_empty) as not_in.
+  pose proof (benumerate_empty) as not_in;
+  unfold BagEnumerateEmpty in not_in.
   destruct (benumerate bempty) as [ | item ? ]; 
     simpl in *;
     [ | exfalso; apply (not_in item) ];
@@ -603,10 +761,10 @@ Instance CachingBagAsBag
                                       ccached_value := cache_updater item container.(ccached_value) |} 
   |}.
 Proof.    
-  simpl; intros; apply binsert_enumerate.
-  simpl; intros; apply benumerate_empty.
-  simpl; intros; apply bstar_search.
-  simpl; intros; apply bfind_correct.
+  unfold BagInsertEnumerate; simpl; intros. apply binsert_enumerate.
+  unfold BagEnumerateEmpty;  simpl; intros; apply benumerate_empty.
+  unfold BagFindStar;        simpl; intros; apply bfind_star.
+  unfold BagFindCorrect;     simpl; intros; apply bfind_correct.
 
   Grab Existential Variables.
 
@@ -1045,8 +1203,9 @@ Defined.
 
 Definition IndexedAlbums :=
   List.fold_left binsert FirstAlbums (@bempty _ _ _ (BagProof SampleIndex)).
+
 (*
-Eval simpl in (SearchTermType AlbumHeading SampleIndex).
+Eval simpl in (SearchTermType SampleIndex).
 Time Eval simpl in (bfind IndexedAlbums (Some 3, (None, (None, [])))).
 Time Eval simpl in (bfind IndexedAlbums (Some 3, (Some 1, (None, [])))).
 Time Eval simpl in (bfind IndexedAlbums (Some 3, (Some 1, (Some "With the Beatles", [])))).
